Examples/AtomicCounter.v
@@ -56,139 +56,9 @@ Definition F := CounterSig.
 Definition VE := tensorSpec lockSpec racyCounterSpec.
 Definition VF := atomicCounterSpec.
 
-Definition Relt := Relt E VE F.
-Definition Prec := Prec E VE F.
-Definition Post := Post E VE F.
-
-Inductive Atomic : Trace (ThreadEvent F) -> Prop :=
-| NilAtomic : Atomic []
-| ConsAtomic {i ρ A} {m : F A} {v : A} :
-  Atomic ρ ->
-  Atomic ((i, CallEv m) :: (i, RetEv m v) :: ρ).
-
-Lemma decideEqNat : forall (n m : nat), {n = m} + {n <> m}.
-fix rec 2.
-intros.
-destruct n, m.
-left.
-congruence.
-right.
-congruence.
-right.
-congruence.
-assert ({n = m} + {n <> m}) by apply rec.
-destruct H.
-left.
-congruence.
-right.
-congruence.
-Qed.
-
-Lemma decideAtomic : forall ρ, {Atomic ρ} + {~(Atomic ρ)}.
-fix rec 1.
-intros.
-destruct ρ.
-left.
-constructor.
-destruct ρ.
-right.
-unfold not.
-intros.
-inversion H.
-destruct t, t0.
-assert ({t = t0} + {t <> t0}) by apply decideEqNat.
-destruct H.
-subst.
-{
-  destruct e, e0.
-  right.
-  unfold not.
-  intros.
-  inversion H.
-  {
-    destruct m, m0.
-    assert ({Atomic ρ} + {~Atomic ρ}) by apply rec.
-    destruct H.
-    left.
-    constructor.
-    easy.
-    right.
-    unfold not.
-    intros.
-    apply n0.
-    inversion H.
-    easy.
-    right.
-    unfold not.
-    intros.
-    dependent destruction H.
-    right.
-    unfold not.
-    intros.
-    dependent destruction H.
-    assert ({Atomic ρ} + {~Atomic ρ}) by apply rec.
-    destruct H.
-    left.
-    constructor.
-    easy.
-    right.
-    unfold not.
-    intros.
-    dependent destruction H.
-    apply n0.
-    easy.
-  }
-  right.
-  unfold not.
-  intros.
-  inversion H.
-  right.
-  unfold not.
-  intros.
-  inversion H.
-}
-right.
-unfold not.
-intros.
-inversion H.
-congruence.
-Qed.
-
-Definition AtomicPrefix (ρ σ : Trace (ThreadEvent F)) : Prop :=
-  exists τ,
-    σ = ρ ++ τ /\
-    Atomic ρ /\
-    ~(Atomic τ).
-
-(*
-left = atomic   right = nonatomic
-acc should always be atomic
-*)
-Fixpoint linAux (acc ρ : Trace (ThreadEvent F)) : Trace (ThreadEvent F) :=
-  match ρ with
-  | [] | [_] => acc
-  | e1 :: e2 :: σ =>
-    match decideAtomic (acc ++ [e1; e2]) with
-    | left _ => linAux (acc ++ [e1; e2]) σ
-    | right _ => acc
-    end
-  end.
-
-Definition lin ρ := linAux [] ρ.
-
-Lemma linSplit ρ σ :
-  ~Atomic σ ->
-  lin (ρ ++ σ) = lin ρ.
-Admitted.
-
-Lemma linSat ρ :
-  lin (lin ρ) = lin ρ.
-Admitted.
-
-Lemma linAtomic ρ :
-  Atomic ρ ->
-  lin ρ = ρ.
-Admitted.
+Definition Relt := Relt VE VF.
+Definition Prec := Prec VE VF.
+Definition Post := Post VE VF.
 
 Definition countState (s : @InterState E F VE) : RacyCounterState :=
   snd (snd s).
@@ -200,114 +70,30 @@ Definition AtomicCounterSteps :
   AtomicCounterState -> Trace (ThreadEvent CounterSig) -> AtomicCounterState -> Prop :=
   Steps AtomicCounterStep.
 
-Lemma atomicTrans m :
-  forall ρ n,
-  AtomicCounterSteps (CounterIdle n) ρ (CounterIdle m) ->
-  Atomic ρ.
-fix rec 1.
-intros.
-destruct ρ.
-constructor.
-destruct ρ.
-dependent destruction H.
-dependent destruction H.
-dependent destruction H0.
-dependent destruction H0.
-do 2 dependent destruction H.
-dependent destruction H0.
-dependent destruction H.
-constructor.
-eapply rec.
-exact H0.
-dependent destruction H0.
-dependent destruction H.
-constructor.
-eapply rec.
-exact H0.
-Qed.
-
-Definition inter i : Relt :=
-  fun s ρ t σ =>
-    exists j,
-      j <> i /\
-      ((InvokeAny atomicCounterImpl j s ρ t σ) \/
-        ReturnAny atomicCounterImpl j s ρ t σ).
-
-
-Definition rely : ThreadName -> Relt :=
-  fun i s ρ t σ =>
-      inter i s ρ t σ \/
-      (lockState s = LockOwned i ->
-        snd s = snd t /\
-        lin ρ = lin σ).
-
-Lemma relyOwned i s ρ t σ :
-  lockState s = LockOwned i ->
-  rely i s ρ t σ ->
-  snd s = snd t /\
-  lin ρ = lin σ.
-unfold countState, lockState.
-destruct s, t, s, s0.
-simpl.
-intros.
-subst.
-destruct H0.
-destruct H.
-destruct H.
-destruct H0.
-do 4 destruct H0.
-destruct H1.
-dependent destruction H3.
-split.
-easy.
-rewrite linSplit.
-easy.
-unfold not.
-intros.
-dependent destruction H1.
-do 4 destruct H0.
-do 4 destruct H1.
-dependent destruction H2.
-easy.
-unfold lockState, countState in H.
-simpl in H.
-apply H.
-easy.
-Qed.
-
-Lemma relyTrans i :
-  rely i ->> rely i ==> rely i.
-unfold rely, inter, sub, subRelt, InvokeAny, TInvoke, ReturnAny, TReturn.
-intros.
-psimpl.
-destruct H, H0.
-psimpl.
-destruct H2, H1.
-Admitted.
-Hint Resolve relyTrans : rely_lemmas.
-
-Lemma relyId i :
-  id ==> rely i.
-unfold sub, subRelt.
-intros.
-destruct H.
-subst.
-right.
-intros.
-easy.
-Qed.
-Hint Resolve relyId : rely_lemmas.
-
-Definition guar : ThreadName -> Relt :=
-  fun i s ρ t σ =>
-      lockState s <> LockOwned i ->
-        snd s = snd t /\
-        lin ρ = lin σ.
-
 Definition invariant : Prec :=
   fun s ρ =>
     exists s',
-      countState s = CounterDSt s'.
+      countState s = CounterDSt s' /\
+      (~(exists i, lockState s = LockOwned i) ->
+        ρ.(PState) = s').
+
+Definition rely : ThreadName -> Relt :=
+  fun i s ρ t σ =>
+    (exists j,
+      i <> j /\
+      InvokeAny atomicCounterImpl j s ρ t σ) \/
+    (exists j,
+      i <> j /\
+      ReturnAny atomicCounterImpl j s ρ t σ) \/
+    (lockState s = LockOwned i ->
+      countState s = countState t /\
+      ρ.(PState) = σ.(PState)).
+
+Definition guar : ThreadName -> Relt :=
+  fun i s ρ t σ =>
+    lockState s <> LockOwned i ->
+      countState s = countState t /\
+      ρ.(PState) = σ.(PState).
 
 Definition precs : ThreadName -> forall Ret, CounterSig Ret -> Prec :=
   fun i Ret m s ρ =>
@@ -325,131 +111,174 @@ repeat lazymatch goal with
 | [ H : ?x = ?y |- ?G ] => try (rewrite H in *; clear H)
 end.
 
-Ltac commit :=
-unfold Commit, precs, guar, invariant, countState, lockState;
-intros;
-psimpl.
+Lemma eqbNeq : forall i j, i <> j -> i =? j = false.
+fix rec 1.
+intros.
+destruct i, j.
+all: congruence || (try easy).
+simpl.
+apply rec.
+congruence.
+Qed.
 
-Lemma listHelpAbsurd {A} {xs ys : list A} {x : A} :
-  [] <> xs ++ x :: ys.
+Lemma precsStable i A m : Stable (rely i) (precs i A m).
+unfold Stable, stablePrec, sub, subPrec, rely.
+intros.
+psimpl.
+destruct H0;
+unfold InvokeAny, ReturnAny, TInvoke, TReturn in *;
+psimpl; steps.
+unfold precs.
+split.
+{
+  split.
+  unfold updThs.
+  simpl.
+  rewrite eqbNeq.
+  do 2 destruct H.
+  all: easy.
+}
+split.
+{
+  unfold precs, invariant, countState, lockState in *.
+  psimpl.
+  exists x.
+  split.
+  easy.
+  intros.
+  apply H8 in H9.
+  congruence.
+}
+unfold lockState.
+simpl.
+destruct H.
+easy.
+destruct H0.
+psimpl.
+{
+  unfold precs, invariant, TIdle in *.
+  psimpl.
+  steps.
+  split.
+  split.
+  unfold updThs.
+  simpl in *.
+  rewrite eqbNeq.
+  easy.
+  easy.
+  easy.
+  split.
+  exists x5.
+  split.
+  easy.
+  intros.
+  all: unfold lockState in *.
+  all: simpl in *.
+  apply H6 in H7.
+  easy.
+  easy.
+}
+unfold precs, invariant, TIdle in *.
+psimpl.
+split.
+split.
 Admitted.
 
-Ltac cond := unfold sub, subRelt, sp, guar, precs, invariant, countState, lockState, TIdle, Util.differ_pointwise in *; intros; psimpl; steps.
-
-Ltac decompose H :=
-lazymatch type of H with
-| InterStep ?i ?s ?ev ?t =>
-  dependent destruction H
-| ?P /\ ?Q  =>
-  let H1 := fresh in
-  let H2 := fresh in
-  destruct H as [H1 H2];
-  decompose H1;
-  decompose H2
-| TInvoke ?impl ?i ?A ?m ?s ?ρ ?t ?σ =>
-  let HI := fresh in
-  let P := fresh "P" in
-  let step := fresh "step" in
-  destruct H as [P HI];
-  destruct HI as [HI step];
-  subst
-| (?P <<- ?Q) ?s ?ρ =>
-  let HI := fresh in
-  let is := fresh "is" in
-  let iρ := fresh "iρ" in
-  let P := fresh "P" in
-  let Q := fresh "Q" in
-  destruct H as [is HI];
-  destruct HI as [iρ HI];
-  destruct HI as [P Q];
-  move is at top;
-  move iρ at top;
-  decompose P;
-  decompose Q
-| ReltToPrec ?P ?s ?ρ =>
-  let HI := fresh in
-  let is := fresh "is" in
-  let iρ := fresh "iρ" in
-  destruct H as [is HI];
-  destruct HI as [iρ HI];
-  move is at top;
-  move iρ at top;
-  decompose HI
-| sp ?impl ?i ?VF ?rel ?prec ?ev ?s ?ρ ?t ?σ =>
-  let HI := fresh in
-  let rs := fresh "rs" in
-  let rρ := fresh "rρ" in
-  let BR := fresh "BR" in
-  let P := fresh "P" in
-  let ss := fresh "ss" in
-  let sρ := fresh "sρ" in
-  let step := fresh "step" in
-  let trace := fresh "trace" in
-  let rw := fresh "rw" in
-  let AR := fresh "AR" in
-  destruct H as [rs HI];
-  destruct HI as [rρ HI];
-  destruct HI as [BR HI];
-  destruct HI as [P HI];
-  destruct HI as [ss HI];
-  destruct HI as [sρ HI];
-  destruct HI as [step HI];
-  destruct HI as [trace HI];
-  destruct HI as [rw AR];
-  move rs at top;
-  move rρ at top;
-  move ss at top;
-  move sρ at top;
-  move P before BR;
-  move trace at bottom;
-  move rw at bottom;
-  dependent destruction step;
-  decompose P
-| _ => idtac
-end.
-
-Ltac prepare H :=
-decompose H;
-repeat lazymatch goal with
-| [ H1 : ?P, H2 : ?P |- ?G] =>
-  clear H1
-end.
+Lemma postsStable i A m : Stable (rely i) (posts i A m).
+Admitted.
 
 Theorem atomicCounterCorrect :
   VerifyImpl VE VF rely guar precs atomicCounterImpl posts.
 unfold VerifyImpl.
 split.
 {
-  unfold guar, rely, sub, subRelt.
-  intros.
-  right.
-  intros.
-  apply H0.
-  congruence.
+  admit.
 }
 split.
-admit.
+{
+  intros.
+  unfold precs, invariant, TIdle.
+  split.
+  repeat split.
+  exists (CounterIdle 0).
+  easy.
+  easy.
+  split.
+  easy.
+  split.
+  eapply precsStable.
+  apply postsStable.
+}
 split.
 admit.
 intros.
 destruct m.
 simpl.
 unfold inc.
-strongBind.
-{
-  unfold sub, subRelt, guar.
-  intros.
-  prepare H.
-  simpl in *.
-  destruct H0.
-  dependent destruction H0.
-  
-}
+eapply SafeBind with
+  (QI:= fun s ρ t σ =>
+    True)
+  (QR:=fun _ s (ρ : Poss VF) t (σ : Poss VF) =>
+    lockState t = LockOwned i /\
+    σ.(PCalls) i = Some (existT _ _ Inc) /\
+    σ.(PRets) i = None /\
+    countState t = countState s /\
+    σ = ρ /\
+    exists k,
+      countState s = CounterDSt (CounterIdle k) /\
+      ρ.(PState) = CounterIdle k).
 admit.
-intros.
-strongBind.
+admit.
+admit.
+split.
+admit.
+eapply SafeBind with
+  (QI:=fun s ρ t (σ : Poss VF) =>
+    lockState t = LockOwned i /\
+    σ.(PCalls) i = Some (existT _ _ Inc) /\
+    σ.(PRets) i = None /\
+    countState t = countState s /\
+    σ = ρ /\
+    exists k,
+      countState s = CounterDSt (CounterIdle k) /\
+      ρ.(PState) = CounterIdle k)
+  (QR:=fun _ s (ρ : Poss VF) t (σ : Poss VF) =>
+    lockState t = LockOwned i /\
+    σ.(PCalls) i = None /\
+    σ.(PRets) i = None /\
+    exists k,
+      ρ.(PState) = CounterIdle k /\
+      countState s = CounterDSt (CounterIdle k) /\
+      σ.(PState) = CounterIdle (S k) /\
+      countState s = CounterDSt (CounterIdle (S k))).
+admit.
+admit.
+admit.
+split.
+{
+  unfold Commit, id.
+  intros.
+  psimpl.
+  steps.
+  dependent destruction H9.
+}
+eapply SafeBind with
+  (QI:=fun s ρ t σ =>
+    True)
+  (QR:=fun _ s (ρ : Poss VF) t (σ : Poss VF) =>
+    lockState t <> LockOwned i /\
+    σ.(PCalls) i = None /\
+    σ.(PRets) i = None /\
+    σ = ρ /\
+    countState t = countState s).
+admit.
+admit.
+admit.
+split.
+admit.
+eapply SafeReturn.
 {
   unfold sub, subRelt.
   intros.
-  decompose H.
+  psimpl.
 }
